<?xml version="1.0"?>
<rdf:RDF xmlns="http://purl.obolibrary.org/obo/ability_type_ontorat.owl#"
     xml:base="http://purl.obolibrary.org/obo/ability_type_ontorat.owl"
     xmlns:rdf="http://www.w3.org/1999/02/22-rdf-syntax-ns#"
     xmlns:owl="http://www.w3.org/2002/07/owl#"
     xmlns:xsd="http://www.w3.org/2001/XMLSchema#"
     xmlns:rdfs="http://www.w3.org/2000/01/rdf-schema#"
     xmlns:obo="http://purl.obolibrary.org/obo/">
    <owl:Ontology rdf:about="http://purl.obolibrary.org/obo/ability_type_ontorat.owl"/>
    


    <!-- 
    ///////////////////////////////////////////////////////////////////////////////////////
    //
    // Annotation properties
    //
    ///////////////////////////////////////////////////////////////////////////////////////
     -->

    <owl:AnnotationProperty rdf:about="http://purl.obolibrary.org/obo/IAO_0000118"/>
    <owl:AnnotationProperty rdf:about="http://purl.obolibrary.org/obo/IAO_0000117"/>
    <owl:AnnotationProperty rdf:about="http://purl.obolibrary.org/obo/IAO_0000119"/>
    <owl:AnnotationProperty rdf:about="http://purl.obolibrary.org/obo/IAO_0000114"/>
    <owl:AnnotationProperty rdf:about="http://purl.obolibrary.org/obo/IAO_0000116"/>
    <owl:AnnotationProperty rdf:about="http://purl.obolibrary.org/obo/IAO_0000115"/>
    <owl:AnnotationProperty rdf:about="http://www.w3.org/2000/01/rdf-schema#seeAlso"/>
    <owl:AnnotationProperty rdf:about="http://purl.obolibrary.org/obo/IAO_0000112"/>
    <owl:AnnotationProperty rdf:about="http://purl.obolibrary.org/obo/IAO_0000111"/>
    <owl:AnnotationProperty rdf:about="http://www.w3.org/2000/01/rdf-schema#comment"/>
    <owl:AnnotationProperty rdf:about="http://purl.obolibrary.org/obo/OccO_00000008"/>
    <owl:AnnotationProperty rdf:about="http://www.w3.org/2000/01/rdf-schema#label"/>
    


    <!-- 
    ///////////////////////////////////////////////////////////////////////////////////////
    //
    // Datatypes
    //
    ///////////////////////////////////////////////////////////////////////////////////////
     -->

    


    <!-- http://www.w3.org/1999/02/22-rdf-syntax-ns#PlainLiteral -->

    <rdfs:Datatype rdf:about="http://www.w3.org/1999/02/22-rdf-syntax-ns#PlainLiteral"/>
    


    <!-- http://www.w3.org/2000/01/rdf-schema#Literal -->

    <rdfs:Datatype rdf:about="http://www.w3.org/2000/01/rdf-schema#Literal"/>
    


    <!-- http://www.w3.org/2001/XMLSchema#float -->

    <rdfs:Datatype rdf:about="http://www.w3.org/2001/XMLSchema#float"/>
    


    <!-- http://www.w3.org/2001/XMLSchema#integer -->

    <rdfs:Datatype rdf:about="http://www.w3.org/2001/XMLSchema#integer"/>
    


    <!-- http://www.w3.org/2001/XMLSchema#nonNegativeInteger -->

    <rdfs:Datatype rdf:about="http://www.w3.org/2001/XMLSchema#nonNegativeInteger"/>
    


    <!-- http://www.w3.org/2001/XMLSchema#string -->

    <rdfs:Datatype rdf:about="http://www.w3.org/2001/XMLSchema#string"/>
    


    <!-- 
    ///////////////////////////////////////////////////////////////////////////////////////
    //
    // Classes
    //
    ///////////////////////////////////////////////////////////////////////////////////////
     -->

    


    <!-- http://purl.obolibrary.org/obo/OccO_00000004 -->

    <owl:Class rdf:about="http://purl.obolibrary.org/obo/OccO_00000004"/>
    


    <!-- http://purl.obolibrary.org/obo/OccO_00000060 -->

    <owl:Class rdf:about="http://purl.obolibrary.org/obo/OccO_00000060">
        <rdfs:label>arm-hand steadiness</rdfs:label>
        <rdfs:subClassOf rdf:resource="http://purl.obolibrary.org/obo/OccO_00000004"/>
        <obo:IAO_0000117>Sam Smith, Oliver He</obo:IAO_0000117>
        <obo:IAO_0000115>The ability to keep your hand and arm steady while moving your arm or while holding your arm and hand in one position.</obo:IAO_0000115>
        <obo:IAO_0000119>https://www.onetonline.org/find/descriptor/browse/1.A/1.A.1/1.A.1.g</obo:IAO_0000119>
        <obo:OccO_00000008>1.A.2.a.1</obo:OccO_00000008>
    </owl:Class>
    


    <!-- http://purl.obolibrary.org/obo/OccO_00000061 -->

    <owl:Class rdf:about="http://purl.obolibrary.org/obo/OccO_00000061">
        <rdfs:label>auditory attention</rdfs:label>
        <rdfs:subClassOf rdf:resource="http://purl.obolibrary.org/obo/OccO_00000004"/>
        <obo:IAO_0000119>https://www.onetonline.org/find/descriptor/browse/1.A/1.A.1/1.A.1.g</obo:IAO_0000119>
        <obo:IAO_0000115>The ability to focus on a single source of sound in the presence of other distracting sounds.</obo:IAO_0000115>
        <obo:IAO_0000117>Sam Smith, Oliver He</obo:IAO_0000117>
        <obo:OccO_00000008>1.A.4.b.2</obo:OccO_00000008>
    </owl:Class>
    


    <!-- http://purl.obolibrary.org/obo/OccO_00000062 -->

    <owl:Class rdf:about="http://purl.obolibrary.org/obo/OccO_00000062">
        <rdfs:label>category flexibility</rdfs:label>
        <rdfs:subClassOf rdf:resource="http://purl.obolibrary.org/obo/OccO_00000004"/>
        <obo:IAO_0000117>Sam Smith, Oliver He</obo:IAO_0000117>
        <obo:IAO_0000115>The ability to generate or use different sets of rules for combining or grouping things in different ways.</obo:IAO_0000115>
        <obo:IAO_0000119>https://www.onetonline.org/find/descriptor/browse/1.A/1.A.1/1.A.1.g</obo:IAO_0000119>
        <obo:OccO_00000008>1.A.1.b.7</obo:OccO_00000008>
    </owl:Class>
    


    <!-- http://purl.obolibrary.org/obo/OccO_00000063 -->

    <owl:Class rdf:about="http://purl.obolibrary.org/obo/OccO_00000063">
        <rdfs:label>control precision</rdfs:label>
        <rdfs:subClassOf rdf:resource="http://purl.obolibrary.org/obo/OccO_00000004"/>
        <obo:OccO_00000008>1.A.2.b.1</obo:OccO_00000008>
        <obo:IAO_0000117>Sam Smith, Oliver He</obo:IAO_0000117>
        <obo:IAO_0000115>The ability to quickly and repeatedly adjust the controls of a machine or a vehicle to exact positions.</obo:IAO_0000115>
        <obo:IAO_0000119>https://www.onetonline.org/find/descriptor/browse/1.A/1.A.1/1.A.1.g</obo:IAO_0000119>
    </owl:Class>
    


    <!-- http://purl.obolibrary.org/obo/OccO_00000064 -->

    <owl:Class rdf:about="http://purl.obolibrary.org/obo/OccO_00000064">
        <rdfs:label>deductive reasoning</rdfs:label>
        <rdfs:subClassOf rdf:resource="http://purl.obolibrary.org/obo/OccO_00000004"/>
        <obo:OccO_00000008>1.A.1.b.4</obo:OccO_00000008>
        <obo:IAO_0000117>Sam Smith, Oliver He</obo:IAO_0000117>
        <obo:IAO_0000115>The ability to apply general rules to specific problems to produce answers that make sense.</obo:IAO_0000115>
        <obo:IAO_0000119>https://www.onetonline.org/find/descriptor/browse/1.A/1.A.1/1.A.1.g</obo:IAO_0000119>
    </owl:Class>
    


    <!-- http://purl.obolibrary.org/obo/OccO_00000065 -->

    <owl:Class rdf:about="http://purl.obolibrary.org/obo/OccO_00000065">
        <rdfs:label>depth perception</rdfs:label>
        <rdfs:subClassOf rdf:resource="http://purl.obolibrary.org/obo/OccO_00000004"/>
        <obo:OccO_00000008>1.A.4.a.6</obo:OccO_00000008>
        <obo:IAO_0000115>The ability to judge which of several objects is closer or farther away from you, or to judge the distance between you and an object.</obo:IAO_0000115>
        <obo:IAO_0000119>https://www.onetonline.org/find/descriptor/browse/1.A/1.A.1/1.A.1.g</obo:IAO_0000119>
        <obo:IAO_0000117>Sam Smith, Oliver He</obo:IAO_0000117>
    </owl:Class>
    


    <!-- http://purl.obolibrary.org/obo/OccO_00000066 -->

    <owl:Class rdf:about="http://purl.obolibrary.org/obo/OccO_00000066">
        <rdfs:label>dynamic flexibility</rdfs:label>
        <rdfs:subClassOf rdf:resource="http://purl.obolibrary.org/obo/OccO_00000004"/>
        <obo:IAO_0000119>https://www.onetonline.org/find/descriptor/browse/1.A/1.A.1/1.A.1.g</obo:IAO_0000119>
        <obo:IAO_0000117>Sam Smith, Oliver He</obo:IAO_0000117>
        <obo:IAO_0000115>The ability to quickly and repeatedly bend, stretch, twist, or reach out with your body, arms, and/or legs.</obo:IAO_0000115>
        <obo:OccO_00000008>1.A.3.c.2</obo:OccO_00000008>
    </owl:Class>
    


    <!-- http://purl.obolibrary.org/obo/OccO_00000067 -->

    <owl:Class rdf:about="http://purl.obolibrary.org/obo/OccO_00000067">
        <rdfs:label>dynamic strength</rdfs:label>
        <rdfs:subClassOf rdf:resource="http://purl.obolibrary.org/obo/OccO_00000004"/>
        <obo:IAO_0000115>The ability to exert muscle force repeatedly or continuously over time. This involves muscular endurance and resistance to muscle fatigue.</obo:IAO_0000115>
        <obo:OccO_00000008>1.A.3.a.3</obo:OccO_00000008>
        <obo:IAO_0000119>https://www.onetonline.org/find/descriptor/browse/1.A/1.A.1/1.A.1.g</obo:IAO_0000119>
        <obo:IAO_0000117>Sam Smith, Oliver He</obo:IAO_0000117>
    </owl:Class>
    


    <!-- http://purl.obolibrary.org/obo/OccO_00000068 -->

    <owl:Class rdf:about="http://purl.obolibrary.org/obo/OccO_00000068">
        <rdfs:label>explosive strength</rdfs:label>
        <rdfs:subClassOf rdf:resource="http://purl.obolibrary.org/obo/OccO_00000004"/>
        <obo:IAO_0000115>The ability to use short bursts of muscle force to propel oneself (as in jumping or sprinting), or to throw an object.</obo:IAO_0000115>
        <obo:IAO_0000119>https://www.onetonline.org/find/descriptor/browse/1.A/1.A.1/1.A.1.g</obo:IAO_0000119>
        <obo:IAO_0000117>Sam Smith, Oliver He</obo:IAO_0000117>
        <obo:OccO_00000008>1.A.3.a.2</obo:OccO_00000008>
    </owl:Class>
    


    <!-- http://purl.obolibrary.org/obo/OccO_00000069 -->

    <owl:Class rdf:about="http://purl.obolibrary.org/obo/OccO_00000069">
        <rdfs:label>extent flexibility</rdfs:label>
        <rdfs:subClassOf rdf:resource="http://purl.obolibrary.org/obo/OccO_00000004"/>
        <obo:OccO_00000008>1.A.3.c.1</obo:OccO_00000008>
        <obo:IAO_0000117>Sam Smith, Oliver He</obo:IAO_0000117>
        <obo:IAO_0000119>https://www.onetonline.org/find/descriptor/browse/1.A/1.A.1/1.A.1.g</obo:IAO_0000119>
        <obo:IAO_0000115>The ability to bend, stretch, twist, or reach with your body, arms, and/or legs.</obo:IAO_0000115>
    </owl:Class>
    


    <!-- http://purl.obolibrary.org/obo/OccO_00000070 -->

    <owl:Class rdf:about="http://purl.obolibrary.org/obo/OccO_00000070">
        <rdfs:label>far vision</rdfs:label>
        <rdfs:subClassOf rdf:resource="http://purl.obolibrary.org/obo/OccO_00000004"/>
        <obo:IAO_0000119>https://www.onetonline.org/find/descriptor/browse/1.A/1.A.1/1.A.1.g</obo:IAO_0000119>
        <obo:IAO_0000115>The ability to see details at a distance.</obo:IAO_0000115>
        <obo:IAO_0000117>Sam Smith, Oliver He</obo:IAO_0000117>
        <obo:OccO_00000008>1.A.4.a.2</obo:OccO_00000008>
    </owl:Class>
    


    <!-- http://purl.obolibrary.org/obo/OccO_00000071 -->

    <owl:Class rdf:about="http://purl.obolibrary.org/obo/OccO_00000071">
        <rdfs:label>finger dexterity</rdfs:label>
        <rdfs:subClassOf rdf:resource="http://purl.obolibrary.org/obo/OccO_00000004"/>
        <obo:OccO_00000008>1.A.2.a.3</obo:OccO_00000008>
        <obo:IAO_0000117>Sam Smith, Oliver He</obo:IAO_0000117>
        <obo:IAO_0000115>The ability to make precisely coordinated movements of the fingers of one or both hands to grasp, manipulate, or assemble very small objects.</obo:IAO_0000115>
        <obo:IAO_0000119>https://www.onetonline.org/find/descriptor/browse/1.A/1.A.1/1.A.1.g</obo:IAO_0000119>
    </owl:Class>
    


    <!-- http://purl.obolibrary.org/obo/OccO_00000072 -->

    <owl:Class rdf:about="http://purl.obolibrary.org/obo/OccO_00000072">
        <rdfs:label>flexibility of closure</rdfs:label>
        <rdfs:subClassOf rdf:resource="http://purl.obolibrary.org/obo/OccO_00000004"/>
        <obo:IAO_0000119>https://www.onetonline.org/find/descriptor/browse/1.A/1.A.1/1.A.1.g</obo:IAO_0000119>
        <obo:OccO_00000008>1.A.1.e.2</obo:OccO_00000008>
        <obo:IAO_0000117>Sam Smith, Oliver He</obo:IAO_0000117>
        <obo:IAO_0000115>The ability to identify or detect a known pattern (a figure, object, word, or sound) that is hidden in other distracting material.</obo:IAO_0000115>
    </owl:Class>
    


    <!-- http://purl.obolibrary.org/obo/OccO_00000073 -->

    <owl:Class rdf:about="http://purl.obolibrary.org/obo/OccO_00000073">
        <rdfs:label>fluency of ideas</rdfs:label>
        <rdfs:subClassOf rdf:resource="http://purl.obolibrary.org/obo/OccO_00000004"/>
        <obo:IAO_0000115>The ability to come up with a number of ideas about a topic (the number of ideas is important, not their quality, correctness, or creativity).</obo:IAO_0000115>
        <obo:IAO_0000117>Sam Smith, Oliver He</obo:IAO_0000117>
        <obo:IAO_0000119>https://www.onetonline.org/find/descriptor/browse/1.A/1.A.1/1.A.1.g</obo:IAO_0000119>
        <obo:OccO_00000008>1.A.1.b.1</obo:OccO_00000008>
    </owl:Class>
    


    <!-- http://purl.obolibrary.org/obo/OccO_00000074 -->

    <owl:Class rdf:about="http://purl.obolibrary.org/obo/OccO_00000074">
        <rdfs:label>glare sensitivity</rdfs:label>
        <rdfs:subClassOf rdf:resource="http://purl.obolibrary.org/obo/OccO_00000004"/>
        <obo:OccO_00000008>1.A.4.a.7</obo:OccO_00000008>
        <obo:IAO_0000115>The ability to see objects in the presence of a glare or bright lighting.</obo:IAO_0000115>
        <obo:IAO_0000117>Sam Smith, Oliver He</obo:IAO_0000117>
        <obo:IAO_0000119>https://www.onetonline.org/find/descriptor/browse/1.A/1.A.1/1.A.1.g</obo:IAO_0000119>
    </owl:Class>
    


    <!-- http://purl.obolibrary.org/obo/OccO_00000075 -->

    <owl:Class rdf:about="http://purl.obolibrary.org/obo/OccO_00000075">
        <rdfs:label>gross body coordination</rdfs:label>
        <rdfs:subClassOf rdf:resource="http://purl.obolibrary.org/obo/OccO_00000004"/>
        <obo:OccO_00000008>1.A.3.c.3</obo:OccO_00000008>
        <obo:IAO_0000115>The ability to coordinate the movement of your arms, legs, and torso together when the whole body is in motion.</obo:IAO_0000115>
        <obo:IAO_0000117>Sam Smith, Oliver He</obo:IAO_0000117>
        <obo:IAO_0000119>https://www.onetonline.org/find/descriptor/browse/1.A/1.A.1/1.A.1.g</obo:IAO_0000119>
    </owl:Class>
    


    <!-- http://purl.obolibrary.org/obo/OccO_00000076 -->

    <owl:Class rdf:about="http://purl.obolibrary.org/obo/OccO_00000076">
        <rdfs:label>gross body equilibrium</rdfs:label>
        <rdfs:subClassOf rdf:resource="http://purl.obolibrary.org/obo/OccO_00000004"/>
        <obo:IAO_0000115>The ability to keep or regain your body balance or stay upright when in an unstable position.</obo:IAO_0000115>
        <obo:OccO_00000008>1.A.3.c.4</obo:OccO_00000008>
        <obo:IAO_0000117>Sam Smith, Oliver He</obo:IAO_0000117>
        <obo:IAO_0000119>https://www.onetonline.org/find/descriptor/browse/1.A/1.A.1/1.A.1.g</obo:IAO_0000119>
    </owl:Class>
    


    <!-- http://purl.obolibrary.org/obo/OccO_00000077 -->

    <owl:Class rdf:about="http://purl.obolibrary.org/obo/OccO_00000077">
        <rdfs:label>hearing sensitivity</rdfs:label>
        <rdfs:subClassOf rdf:resource="http://purl.obolibrary.org/obo/OccO_00000004"/>
        <obo:IAO_0000115>The ability to detect or tell the differences between sounds that vary in pitch and loudness.</obo:IAO_0000115>
        <obo:IAO_0000119>https://www.onetonline.org/find/descriptor/browse/1.A/1.A.1/1.A.1.g</obo:IAO_0000119>
        <obo:OccO_00000008>1.A.4.b.1</obo:OccO_00000008>
        <obo:IAO_0000117>Sam Smith, Oliver He</obo:IAO_0000117>
    </owl:Class>
    


    <!-- http://purl.obolibrary.org/obo/OccO_00000078 -->

    <owl:Class rdf:about="http://purl.obolibrary.org/obo/OccO_00000078">
        <rdfs:label>inductive reasoning</rdfs:label>
        <rdfs:subClassOf rdf:resource="http://purl.obolibrary.org/obo/OccO_00000004"/>
        <obo:IAO_0000119>https://www.onetonline.org/find/descriptor/browse/1.A/1.A.1/1.A.1.g</obo:IAO_0000119>
        <obo:IAO_0000115>The ability to combine pieces of information to form general rules or conclusions (includes finding a relationship among seemingly unrelated events).</obo:IAO_0000115>
        <obo:IAO_0000117>Sam Smith, Oliver He</obo:IAO_0000117>
        <obo:OccO_00000008>1.A.1.b.5</obo:OccO_00000008>
    </owl:Class>
    


    <!-- http://purl.obolibrary.org/obo/OccO_00000079 -->

    <owl:Class rdf:about="http://purl.obolibrary.org/obo/OccO_00000079">
        <rdfs:label>information ordering</rdfs:label>
        <rdfs:subClassOf rdf:resource="http://purl.obolibrary.org/obo/OccO_00000004"/>
        <obo:IAO_0000115>The ability to arrange things or actions in a certain order or pattern according to a specific rule or set of rules (e.g., patterns of numbers, letters, words, pictures, mathematical operations).</obo:IAO_0000115>
        <obo:IAO_0000119>https://www.onetonline.org/find/descriptor/browse/1.A/1.A.1/1.A.1.g</obo:IAO_0000119>
        <obo:OccO_00000008>1.A.1.b.6</obo:OccO_00000008>
        <obo:IAO_0000117>Sam Smith, Oliver He</obo:IAO_0000117>
    </owl:Class>
    


    <!-- http://purl.obolibrary.org/obo/OccO_00000080 -->

    <owl:Class rdf:about="http://purl.obolibrary.org/obo/OccO_00000080">
        <rdfs:label>manual dexterity</rdfs:label>
        <rdfs:subClassOf rdf:resource="http://purl.obolibrary.org/obo/OccO_00000004"/>
        <obo:IAO_0000119>https://www.onetonline.org/find/descriptor/browse/1.A/1.A.1/1.A.1.g</obo:IAO_0000119>
        <obo:IAO_0000115>The ability to quickly move your hand, your hand together with your arm, or your two hands to grasp, manipulate, or assemble objects.</obo:IAO_0000115>
        <obo:OccO_00000008>1.A.2.a.2</obo:OccO_00000008>
        <obo:IAO_0000117>Sam Smith, Oliver He</obo:IAO_0000117>
    </owl:Class>
    


    <!-- http://purl.obolibrary.org/obo/OccO_00000081 -->

    <owl:Class rdf:about="http://purl.obolibrary.org/obo/OccO_00000081">
        <rdfs:label>mathematical reasoning</rdfs:label>
        <rdfs:subClassOf rdf:resource="http://purl.obolibrary.org/obo/OccO_00000004"/>
        <obo:IAO_0000119>https://www.onetonline.org/find/descriptor/browse/1.A/1.A.1/1.A.1.g</obo:IAO_0000119>
        <obo:IAO_0000117>Sam Smith, Oliver He</obo:IAO_0000117>
        <obo:IAO_0000115>The ability to choose the right mathematical methods or formulas to solve a problem.</obo:IAO_0000115>
        <obo:OccO_00000008>1.A.1.c.1</obo:OccO_00000008>
    </owl:Class>
    


    <!-- http://purl.obolibrary.org/obo/OccO_00000082 -->

    <owl:Class rdf:about="http://purl.obolibrary.org/obo/OccO_00000082">
        <rdfs:label>memorization</rdfs:label>
        <rdfs:subClassOf rdf:resource="http://purl.obolibrary.org/obo/OccO_00000004"/>
        <obo:IAO_0000117>Sam Smith, Oliver He</obo:IAO_0000117>
        <obo:IAO_0000119>https://www.onetonline.org/find/descriptor/browse/1.A/1.A.1/1.A.1.g</obo:IAO_0000119>
        <obo:IAO_0000115>The ability to remember information such as words, numbers, pictures, and procedures.</obo:IAO_0000115>
        <obo:OccO_00000008>1.A.1.d.1</obo:OccO_00000008>
    </owl:Class>
    


    <!-- http://purl.obolibrary.org/obo/OccO_00000083 -->

    <owl:Class rdf:about="http://purl.obolibrary.org/obo/OccO_00000083">
        <rdfs:label>multilimb coordination</rdfs:label>
        <rdfs:subClassOf rdf:resource="http://purl.obolibrary.org/obo/OccO_00000004"/>
        <obo:IAO_0000115>The ability to coordinate two or more limbs (for example, two arms, two legs, or one leg and one arm) while sitting, standing, or lying down. It does not involve performing the activities while the whole body is in motion.</obo:IAO_0000115>
        <obo:IAO_0000119>https://www.onetonline.org/find/descriptor/browse/1.A/1.A.1/1.A.1.g</obo:IAO_0000119>
        <obo:IAO_0000117>Sam Smith, Oliver He</obo:IAO_0000117>
        <obo:OccO_00000008>1.A.2.b.2</obo:OccO_00000008>
    </owl:Class>
    


    <!-- http://purl.obolibrary.org/obo/OccO_00000084 -->

    <owl:Class rdf:about="http://purl.obolibrary.org/obo/OccO_00000084">
        <rdfs:label>near vision</rdfs:label>
        <rdfs:subClassOf rdf:resource="http://purl.obolibrary.org/obo/OccO_00000004"/>
        <obo:IAO_0000117>Sam Smith, Oliver He</obo:IAO_0000117>
        <obo:IAO_0000119>https://www.onetonline.org/find/descriptor/browse/1.A/1.A.1/1.A.1.g</obo:IAO_0000119>
        <obo:OccO_00000008>1.A.4.a.1</obo:OccO_00000008>
        <obo:IAO_0000115>The ability to see details at close range (within a few feet of the observer).</obo:IAO_0000115>
    </owl:Class>
    


    <!-- http://purl.obolibrary.org/obo/OccO_00000085 -->

    <owl:Class rdf:about="http://purl.obolibrary.org/obo/OccO_00000085">
        <rdfs:label>night vision</rdfs:label>
        <rdfs:subClassOf rdf:resource="http://purl.obolibrary.org/obo/OccO_00000004"/>
        <obo:IAO_0000115>The ability to see under low-light conditions.</obo:IAO_0000115>
        <obo:OccO_00000008>1.A.4.a.4</obo:OccO_00000008>
        <obo:IAO_0000117>Sam Smith, Oliver He</obo:IAO_0000117>
        <obo:IAO_0000119>https://www.onetonline.org/find/descriptor/browse/1.A/1.A.1/1.A.1.g</obo:IAO_0000119>
    </owl:Class>
    


    <!-- http://purl.obolibrary.org/obo/OccO_00000086 -->

    <owl:Class rdf:about="http://purl.obolibrary.org/obo/OccO_00000086">
        <rdfs:label>number facility</rdfs:label>
        <rdfs:subClassOf rdf:resource="http://purl.obolibrary.org/obo/OccO_00000004"/>
        <obo:IAO_0000117>Sam Smith, Oliver He</obo:IAO_0000117>
        <obo:IAO_0000119>https://www.onetonline.org/find/descriptor/browse/1.A/1.A.1/1.A.1.g</obo:IAO_0000119>
        <obo:IAO_0000115>The ability to add, subtract, multiply, or divide quickly and correctly.</obo:IAO_0000115>
        <obo:OccO_00000008>1.A.1.c.2</obo:OccO_00000008>
    </owl:Class>
    


    <!-- http://purl.obolibrary.org/obo/OccO_00000087 -->

    <owl:Class rdf:about="http://purl.obolibrary.org/obo/OccO_00000087">
        <rdfs:label>oral comprehension</rdfs:label>
        <rdfs:subClassOf rdf:resource="http://purl.obolibrary.org/obo/OccO_00000004"/>
        <obo:OccO_00000008>1.A.1.a.1</obo:OccO_00000008>
        <obo:IAO_0000115>The ability to listen to and understand information and ideas presented through spoken words and sentences.</obo:IAO_0000115>
        <obo:IAO_0000117>Sam Smith, Oliver He</obo:IAO_0000117>
        <obo:IAO_0000119>https://www.onetonline.org/find/descriptor/browse/1.A/1.A.1/1.A.1.g</obo:IAO_0000119>
    </owl:Class>
    


    <!-- http://purl.obolibrary.org/obo/OccO_00000088 -->

    <owl:Class rdf:about="http://purl.obolibrary.org/obo/OccO_00000088">
        <rdfs:label>oral expression</rdfs:label>
        <rdfs:subClassOf rdf:resource="http://purl.obolibrary.org/obo/OccO_00000004"/>
        <obo:IAO_0000119>https://www.onetonline.org/find/descriptor/browse/1.A/1.A.1/1.A.1.g</obo:IAO_0000119>
        <obo:IAO_0000115>The ability to communicate information and ideas in speaking so others will understand.</obo:IAO_0000115>
        <obo:IAO_0000117>Sam Smith, Oliver He</obo:IAO_0000117>
        <obo:OccO_00000008>1.A.1.a.3</obo:OccO_00000008>
    </owl:Class>
    


    <!-- http://purl.obolibrary.org/obo/OccO_00000089 -->

    <owl:Class rdf:about="http://purl.obolibrary.org/obo/OccO_00000089">
        <rdfs:label>originality</rdfs:label>
        <rdfs:subClassOf rdf:resource="http://purl.obolibrary.org/obo/OccO_00000004"/>
        <obo:OccO_00000008>1.A.1.b.2</obo:OccO_00000008>
        <obo:IAO_0000119>https://www.onetonline.org/find/descriptor/browse/1.A/1.A.1/1.A.1.g</obo:IAO_0000119>
        <obo:IAO_0000115>The ability to come up with unusual or clever ideas about a given topic or situation, or to develop creative ways to solve a problem.</obo:IAO_0000115>
        <obo:IAO_0000117>Sam Smith, Oliver He</obo:IAO_0000117>
    </owl:Class>
    


    <!-- http://purl.obolibrary.org/obo/OccO_00000090 -->

    <owl:Class rdf:about="http://purl.obolibrary.org/obo/OccO_00000090">
        <rdfs:label>perceptual speed</rdfs:label>
        <rdfs:subClassOf rdf:resource="http://purl.obolibrary.org/obo/OccO_00000004"/>
        <obo:IAO_0000119>https://www.onetonline.org/find/descriptor/browse/1.A/1.A.1/1.A.1.g</obo:IAO_0000119>
        <obo:IAO_0000117>Sam Smith, Oliver He</obo:IAO_0000117>
        <obo:IAO_0000115>The ability to quickly and accurately compare similarities and differences among sets of letters, numbers, objects, pictures, or patterns. The things to be compared may be presented at the same time or one after the other. This ability also includes comparing a presented object with a remembered object.</obo:IAO_0000115>
        <obo:OccO_00000008>1.A.1.e.3</obo:OccO_00000008>
    </owl:Class>
    


    <!-- http://purl.obolibrary.org/obo/OccO_00000091 -->

    <owl:Class rdf:about="http://purl.obolibrary.org/obo/OccO_00000091">
        <rdfs:label>peripheral vision</rdfs:label>
        <rdfs:subClassOf rdf:resource="http://purl.obolibrary.org/obo/OccO_00000004"/>
        <obo:OccO_00000008>1.A.4.a.5</obo:OccO_00000008>
        <obo:IAO_0000115>The ability to see objects or movement of objects to one&#39;s side when the eyes are looking ahead.</obo:IAO_0000115>
        <obo:IAO_0000117>Sam Smith, Oliver He</obo:IAO_0000117>
        <obo:IAO_0000119>https://www.onetonline.org/find/descriptor/browse/1.A/1.A.1/1.A.1.g</obo:IAO_0000119>
    </owl:Class>
    


    <!-- http://purl.obolibrary.org/obo/OccO_00000092 -->

    <owl:Class rdf:about="http://purl.obolibrary.org/obo/OccO_00000092">
        <rdfs:label>problem sensitivity</rdfs:label>
        <rdfs:subClassOf rdf:resource="http://purl.obolibrary.org/obo/OccO_00000004"/>
        <obo:IAO_0000115>The ability to tell when something is wrong or is likely to go wrong. It does not involve solving the problem, only recognizing that there is a problem.</obo:IAO_0000115>
        <obo:IAO_0000119>https://www.onetonline.org/find/descriptor/browse/1.A/1.A.1/1.A.1.g</obo:IAO_0000119>
        <obo:IAO_0000117>Sam Smith, Oliver He</obo:IAO_0000117>
        <obo:OccO_00000008>1.A.1.b.3</obo:OccO_00000008>
    </owl:Class>
    


    <!-- http://purl.obolibrary.org/obo/OccO_00000093 -->

    <owl:Class rdf:about="http://purl.obolibrary.org/obo/OccO_00000093">
        <rdfs:label>rate control</rdfs:label>
        <rdfs:subClassOf rdf:resource="http://purl.obolibrary.org/obo/OccO_00000004"/>
        <obo:IAO_0000117>Sam Smith, Oliver He</obo:IAO_0000117>
        <obo:OccO_00000008>1.A.2.b.4</obo:OccO_00000008>
        <obo:IAO_0000119>https://www.onetonline.org/find/descriptor/browse/1.A/1.A.1/1.A.1.g</obo:IAO_0000119>
        <obo:IAO_0000115>The ability to time your movements or the movement of a piece of equipment in anticipation of changes in the speed and/or direction of a moving object or scene.</obo:IAO_0000115>
    </owl:Class>
    


    <!-- http://purl.obolibrary.org/obo/OccO_00000094 -->

    <owl:Class rdf:about="http://purl.obolibrary.org/obo/OccO_00000094">
        <rdfs:label>reaction time</rdfs:label>
        <rdfs:subClassOf rdf:resource="http://purl.obolibrary.org/obo/OccO_00000004"/>
        <obo:IAO_0000119>https://www.onetonline.org/find/descriptor/browse/1.A/1.A.1/1.A.1.g</obo:IAO_0000119>
        <obo:IAO_0000117>Sam Smith, Oliver He</obo:IAO_0000117>
        <obo:OccO_00000008>1.A.2.c.1</obo:OccO_00000008>
        <obo:IAO_0000115>The ability to quickly respond (with the hand, finger, or foot) to a signal (sound, light, picture) when it appears.</obo:IAO_0000115>
    </owl:Class>
    


    <!-- http://purl.obolibrary.org/obo/OccO_00000095 -->

    <owl:Class rdf:about="http://purl.obolibrary.org/obo/OccO_00000095">
        <rdfs:label>response orientation</rdfs:label>
        <rdfs:subClassOf rdf:resource="http://purl.obolibrary.org/obo/OccO_00000004"/>
        <obo:IAO_0000117>Sam Smith, Oliver He</obo:IAO_0000117>
        <obo:OccO_00000008>1.A.2.b.3</obo:OccO_00000008>
        <obo:IAO_0000119>https://www.onetonline.org/find/descriptor/browse/1.A/1.A.1/1.A.1.g</obo:IAO_0000119>
        <obo:IAO_0000115>The ability to choose quickly between two or more movements in response to two or more different signals (lights, sounds, pictures). It includes the speed with which the correct response is started with the hand, foot, or other body part.</obo:IAO_0000115>
    </owl:Class>
    


    <!-- http://purl.obolibrary.org/obo/OccO_00000096 -->

    <owl:Class rdf:about="http://purl.obolibrary.org/obo/OccO_00000096">
        <rdfs:label>selective attention</rdfs:label>
        <rdfs:subClassOf rdf:resource="http://purl.obolibrary.org/obo/OccO_00000004"/>
        <obo:OccO_00000008>1.A.1.g.1</obo:OccO_00000008>
        <obo:IAO_0000119>https://www.onetonline.org/find/descriptor/browse/1.A/1.A.1/1.A.1.g</obo:IAO_0000119>
        <obo:IAO_0000117>Sam Smith, Oliver He</obo:IAO_0000117>
        <obo:IAO_0000115>The ability to concentrate on a task over a period of time without being distracted.</obo:IAO_0000115>
    </owl:Class>
    


    <!-- http://purl.obolibrary.org/obo/OccO_00000097 -->

    <owl:Class rdf:about="http://purl.obolibrary.org/obo/OccO_00000097">
        <rdfs:label>sound localization</rdfs:label>
        <rdfs:subClassOf rdf:resource="http://purl.obolibrary.org/obo/OccO_00000004"/>
        <obo:IAO_0000119>https://www.onetonline.org/find/descriptor/browse/1.A/1.A.1/1.A.1.g</obo:IAO_0000119>
        <obo:IAO_0000115>The ability to tell the direction from which a sound originated.</obo:IAO_0000115>
        <obo:IAO_0000117>Sam Smith, Oliver He</obo:IAO_0000117>
        <obo:OccO_00000008>1.A.4.b.3</obo:OccO_00000008>
    </owl:Class>
    


    <!-- http://purl.obolibrary.org/obo/OccO_00000098 -->

    <owl:Class rdf:about="http://purl.obolibrary.org/obo/OccO_00000098">
        <rdfs:label>spatial orientation</rdfs:label>
        <rdfs:subClassOf rdf:resource="http://purl.obolibrary.org/obo/OccO_00000004"/>
        <obo:OccO_00000008>1.A.1.f.1</obo:OccO_00000008>
        <obo:IAO_0000119>https://www.onetonline.org/find/descriptor/browse/1.A/1.A.1/1.A.1.g</obo:IAO_0000119>
        <obo:IAO_0000115>The ability to know your location in relation to the environment or to know where other objects are in relation to you.</obo:IAO_0000115>
        <obo:IAO_0000117>Sam Smith, Oliver He</obo:IAO_0000117>
    </owl:Class>
    


    <!-- http://purl.obolibrary.org/obo/OccO_00000099 -->

    <owl:Class rdf:about="http://purl.obolibrary.org/obo/OccO_00000099">
        <rdfs:label>speech clarity</rdfs:label>
        <rdfs:subClassOf rdf:resource="http://purl.obolibrary.org/obo/OccO_00000004"/>
        <obo:IAO_0000115>The ability to speak clearly so others can understand you.</obo:IAO_0000115>
        <obo:IAO_0000117>Sam Smith, Oliver He</obo:IAO_0000117>
        <obo:IAO_0000119>https://www.onetonline.org/find/descriptor/browse/1.A/1.A.1/1.A.1.g</obo:IAO_0000119>
        <obo:OccO_00000008>1.A.4.b.5</obo:OccO_00000008>
    </owl:Class>
    


    <!-- http://purl.obolibrary.org/obo/OccO_00000100 -->

    <owl:Class rdf:about="http://purl.obolibrary.org/obo/OccO_00000100">
        <rdfs:label>speech recognition</rdfs:label>
        <rdfs:subClassOf rdf:resource="http://purl.obolibrary.org/obo/OccO_00000004"/>
        <obo:OccO_00000008>1.A.4.b.4</obo:OccO_00000008>
        <obo:IAO_0000119>https://www.onetonline.org/find/descriptor/browse/1.A/1.A.1/1.A.1.g</obo:IAO_0000119>
        <obo:IAO_0000117>Sam Smith, Oliver He</obo:IAO_0000117>
        <obo:IAO_0000115>The ability to identify and understand the speech of another person.</obo:IAO_0000115>
    </owl:Class>
    


    <!-- http://purl.obolibrary.org/obo/OccO_00000101 -->

    <owl:Class rdf:about="http://purl.obolibrary.org/obo/OccO_00000101">
        <rdfs:label>speed of closure</rdfs:label>
        <rdfs:subClassOf rdf:resource="http://purl.obolibrary.org/obo/OccO_00000004"/>
        <obo:IAO_0000119>https://www.onetonline.org/find/descriptor/browse/1.A/1.A.1/1.A.1.g</obo:IAO_0000119>
        <obo:IAO_0000115>The ability to quickly make sense of, combine, and organize information into meaningful patterns.</obo:IAO_0000115>
        <obo:OccO_00000008>1.A.1.e.1</obo:OccO_00000008>
        <obo:IAO_0000117>Sam Smith, Oliver He</obo:IAO_0000117>
    </owl:Class>
    


    <!-- http://purl.obolibrary.org/obo/OccO_00000102 -->

    <owl:Class rdf:about="http://purl.obolibrary.org/obo/OccO_00000102">
        <rdfs:label>speed of limb movement</rdfs:label>
        <rdfs:subClassOf rdf:resource="http://purl.obolibrary.org/obo/OccO_00000004"/>
        <obo:OccO_00000008>1.A.2.c.3</obo:OccO_00000008>
        <obo:IAO_0000117>Sam Smith, Oliver He</obo:IAO_0000117>
        <obo:IAO_0000115>The ability to quickly move the arms and legs.</obo:IAO_0000115>
        <obo:IAO_0000119>https://www.onetonline.org/find/descriptor/browse/1.A/1.A.1/1.A.1.g</obo:IAO_0000119>
    </owl:Class>
    


    <!-- http://purl.obolibrary.org/obo/OccO_00000103 -->

    <owl:Class rdf:about="http://purl.obolibrary.org/obo/OccO_00000103">
        <rdfs:label>stamina</rdfs:label>
        <rdfs:subClassOf rdf:resource="http://purl.obolibrary.org/obo/OccO_00000004"/>
        <obo:IAO_0000117>Sam Smith, Oliver He</obo:IAO_0000117>
        <obo:OccO_00000008>1.A.3.b.1</obo:OccO_00000008>
        <obo:IAO_0000119>https://www.onetonline.org/find/descriptor/browse/1.A/1.A.1/1.A.1.g</obo:IAO_0000119>
        <obo:IAO_0000115>The ability to exert yourself physically over long periods of time without getting winded or out of breath.</obo:IAO_0000115>
    </owl:Class>
    


    <!-- http://purl.obolibrary.org/obo/OccO_00000104 -->

    <owl:Class rdf:about="http://purl.obolibrary.org/obo/OccO_00000104">
        <rdfs:label>static strength</rdfs:label>
        <rdfs:subClassOf rdf:resource="http://purl.obolibrary.org/obo/OccO_00000004"/>
        <obo:IAO_0000117>Sam Smith, Oliver He</obo:IAO_0000117>
        <obo:OccO_00000008>1.A.3.a.1</obo:OccO_00000008>
        <obo:IAO_0000119>https://www.onetonline.org/find/descriptor/browse/1.A/1.A.1/1.A.1.g</obo:IAO_0000119>
        <obo:IAO_0000115>The ability to exert maximum muscle force to lift, push, pull, or carry objects.</obo:IAO_0000115>
    </owl:Class>
    


    <!-- http://purl.obolibrary.org/obo/OccO_00000105 -->

    <owl:Class rdf:about="http://purl.obolibrary.org/obo/OccO_00000105">
        <rdfs:label>time sharing</rdfs:label>
        <rdfs:subClassOf rdf:resource="http://purl.obolibrary.org/obo/OccO_00000004"/>
        <obo:IAO_0000115>The ability to shift back and forth between two or more activities or sources of information (such as speech, sounds, touch, or other sources).</obo:IAO_0000115>
        <obo:IAO_0000117>Sam Smith, Oliver He</obo:IAO_0000117>
        <obo:IAO_0000119>https://www.onetonline.org/find/descriptor/browse/1.A/1.A.1/1.A.1.g</obo:IAO_0000119>
        <obo:OccO_00000008>1.A.1.g.2</obo:OccO_00000008>
    </owl:Class>
    


    <!-- http://purl.obolibrary.org/obo/OccO_00000106 -->

    <owl:Class rdf:about="http://purl.obolibrary.org/obo/OccO_00000106">
        <rdfs:label>trunk strength</rdfs:label>
        <rdfs:subClassOf rdf:resource="http://purl.obolibrary.org/obo/OccO_00000004"/>
        <obo:IAO_0000115>The ability to use your abdominal and lower back muscles to support part of the body repeatedly or continuously over time without &quot;giving out&quot; or fatiguing.</obo:IAO_0000115>
        <obo:OccO_00000008>1.A.3.a.4</obo:OccO_00000008>
        <obo:IAO_0000119>https://www.onetonline.org/find/descriptor/browse/1.A/1.A.1/1.A.1.g</obo:IAO_0000119>
        <obo:IAO_0000117>Sam Smith, Oliver He</obo:IAO_0000117>
    </owl:Class>
    


    <!-- http://purl.obolibrary.org/obo/OccO_00000107 -->

    <owl:Class rdf:about="http://purl.obolibrary.org/obo/OccO_00000107">
        <rdfs:label>visual color discrimination</rdfs:label>
        <rdfs:subClassOf rdf:resource="http://purl.obolibrary.org/obo/OccO_00000004"/>
        <obo:OccO_00000008>1.A.4.a.3</obo:OccO_00000008>
        <obo:IAO_0000115>The ability to match or detect differences between colors, including shades of color and brightness.</obo:IAO_0000115>
        <obo:IAO_0000119>https://www.onetonline.org/find/descriptor/browse/1.A/1.A.1/1.A.1.g</obo:IAO_0000119>
        <obo:IAO_0000117>Sam Smith, Oliver He</obo:IAO_0000117>
    </owl:Class>
    


    <!-- http://purl.obolibrary.org/obo/OccO_00000108 -->

    <owl:Class rdf:about="http://purl.obolibrary.org/obo/OccO_00000108">
        <rdfs:label>visualization</rdfs:label>
        <rdfs:subClassOf rdf:resource="http://purl.obolibrary.org/obo/OccO_00000004"/>
        <obo:IAO_0000119>https://www.onetonline.org/find/descriptor/browse/1.A/1.A.1/1.A.1.g</obo:IAO_0000119>
        <obo:OccO_00000008>1.A.1.f.2</obo:OccO_00000008>
        <obo:IAO_0000117>Sam Smith, Oliver He</obo:IAO_0000117>
        <obo:IAO_0000115>The ability to imagine how something will look after it is moved around or when its parts are moved or rearranged.</obo:IAO_0000115>
    </owl:Class>
    


    <!-- http://purl.obolibrary.org/obo/OccO_00000109 -->

    <owl:Class rdf:about="http://purl.obolibrary.org/obo/OccO_00000109">
        <rdfs:label>wrist-finger speed</rdfs:label>
        <rdfs:subClassOf rdf:resource="http://purl.obolibrary.org/obo/OccO_00000004"/>
        <obo:OccO_00000008>1.A.2.c.2</obo:OccO_00000008>
        <obo:IAO_0000117>Sam Smith, Oliver He</obo:IAO_0000117>
        <obo:IAO_0000115>The ability to make fast, simple, repeated movements of the fingers, hands, and wrists.</obo:IAO_0000115>
        <obo:IAO_0000119>https://www.onetonline.org/find/descriptor/browse/1.A/1.A.1/1.A.1.g</obo:IAO_0000119>
    </owl:Class>
    


    <!-- http://purl.obolibrary.org/obo/OccO_00000110 -->

    <owl:Class rdf:about="http://purl.obolibrary.org/obo/OccO_00000110">
        <rdfs:label>written comprehension</rdfs:label>
        <rdfs:subClassOf rdf:resource="http://purl.obolibrary.org/obo/OccO_00000004"/>
        <obo:IAO_0000119>https://www.onetonline.org/find/descriptor/browse/1.A/1.A.1/1.A.1.g</obo:IAO_0000119>
        <obo:IAO_0000115>The ability to read and understand information and ideas presented in writing.</obo:IAO_0000115>
        <obo:IAO_0000117>Sam Smith, Oliver He</obo:IAO_0000117>
        <obo:OccO_00000008>1.A.1.a.2</obo:OccO_00000008>
    </owl:Class>
    


    <!-- http://purl.obolibrary.org/obo/OccO_00000111 -->

    <owl:Class rdf:about="http://purl.obolibrary.org/obo/OccO_00000111">
        <rdfs:label>written expression</rdfs:label>
        <rdfs:subClassOf rdf:resource="http://purl.obolibrary.org/obo/OccO_00000004"/>
        <obo:IAO_0000115>The ability to communicate information and ideas in writing so others will understand.</obo:IAO_0000115>
        <obo:OccO_00000008>1.A.1.a.4</obo:OccO_00000008>
        <obo:IAO_0000119>https://www.onetonline.org/find/descriptor/browse/1.A/1.A.1/1.A.1.g</obo:IAO_0000119>
        <obo:IAO_0000117>Sam Smith, Oliver He</obo:IAO_0000117>
    </owl:Class>
</rdf:RDF>



<!-- Generated by the OWL API (version 1.3.5.1016) http://owlapi.sourceforge.net -->

